

# Algorithm

Good: Finiteness  
Definiteness  
Input/Output  
Effectiveness

## Fixed point arithmetic

1. Signed integer used  
 $M=8+21=00010101$
2. One's complement  
 $M=8, +21: 00010101$   
 $-21: 11101010$
3. Two's complement  
 $M=8, +21: 00010101$   
 $-21: 11101011$

1. Finite urn (red/blue balls)  
red + p, blue - q, p + q = 1  
 $N(t) = N(0) + \sum_{s=0}^{t-1} (p - q)$   
 $E(N(t)) = E(N(0)) + t(p - q)$   
 $E(N(t)) = E(N(0)) + t(p - q)$   
 $E(N(t)) = E(N(0)) + t(p - q)$

2. Random walk  
 $X(t) = X(0) + \sum_{s=0}^{t-1} \epsilon_s$   
 $E(X(t)) = E(X(0)) + t E(\epsilon)$   
 $E(X(t)) = E(X(0)) + t E(\epsilon)$   
 $E(X(t)) = E(X(0)) + t E(\epsilon)$

3. Incomplete Beta Function  
 $I_x(a,b) = \frac{1}{B(a,b)} \int_0^x t^{a-1} (1-t)^{b-1} dt$   
 $I_x(a,b) = \frac{1}{B(a,b)} \int_0^x t^{a-1} (1-t)^{b-1} dt$   
 $I_x(a,b) = \frac{1}{B(a,b)} \int_0^x t^{a-1} (1-t)^{b-1} dt$

4. Distribution Connections  
 $X \sim \text{Gamma}(a, \lambda)$   
 $Y \sim \text{Gamma}(b, \lambda)$   
 $X+Y \sim \text{Gamma}(a+b, \lambda)$   
 $X \sim \text{Gamma}(a, \lambda)$   
 $Y \sim \text{Gamma}(b, \lambda)$   
 $X+Y \sim \text{Gamma}(a+b, \lambda)$

5. Finite Taylor Expansion  
 $f(x) = \sum_{k=0}^n \frac{f^{(k)}(a)}{k!} (x-a)^k + R_n(x)$   
 $R_n(x) = \frac{f^{(n+1)}(\xi)}{(n+1)!} (x-a)^{n+1}$   
 $R_n(x) = \frac{f^{(n+1)}(\xi)}{(n+1)!} (x-a)^{n+1}$

6. Matrix Norms  
 $\|A\|_1 = \sum_{j=1}^n \sum_{i=1}^m |a_{ij}|$   
 $\|A\|_2 = \sqrt{\lambda_{\max}(A^T A)}$   
 $\|A\|_\infty = \max_{i=1, \dots, m} \sum_{j=1}^n |a_{ij}|$   
 $\|A\|_F = \sqrt{\sum_{i,j} |a_{ij}|^2}$

7. Linear Regression  
 $\beta = \arg \min_{\beta} \sum_{i=1}^n (y_i - x_i^T \beta)^2$   
 $\beta = \arg \min_{\beta} \sum_{i=1}^n (y_i - x_i^T \beta)^2$   
 $\beta = \arg \min_{\beta} \sum_{i=1}^n (y_i - x_i^T \beta)^2$

8. Normal Equations  
 $X^T X \beta = X^T y$   
 $\beta = (X^T X)^{-1} X^T y$   
 $\beta = (X^T X)^{-1} X^T y$

9. Polynomial number system  
 $\mathbb{Z}_m[x]$   
 $\mathbb{Z}_m[x] = \{a_0 + a_1 x + \dots + a_n x^n \mid a_i \in \mathbb{Z}_m\}$   
 $\mathbb{Z}_m[x] = \{a_0 + a_1 x + \dots + a_n x^n \mid a_i \in \mathbb{Z}_m\}$

10. Trade-off between storage  
(cost) and computation  
(time/resources)  
 $\mathbb{Z}_m[x] = \{a_0 + a_1 x + \dots + a_n x^n \mid a_i \in \mathbb{Z}_m\}$   
 $\mathbb{Z}_m[x] = \{a_0 + a_1 x + \dots + a_n x^n \mid a_i \in \mathbb{Z}_m\}$

11. Integer Arithmetic  
 $\mathbb{Z}_m[x] = \{a_0 + a_1 x + \dots + a_n x^n \mid a_i \in \mathbb{Z}_m\}$   
 $\mathbb{Z}_m[x] = \{a_0 + a_1 x + \dots + a_n x^n \mid a_i \in \mathbb{Z}_m\}$   
 $\mathbb{Z}_m[x] = \{a_0 + a_1 x + \dots + a_n x^n \mid a_i \in \mathbb{Z}_m\}$

12. Networks: random matrix  
 $A \in \mathbb{R}^{n \times n}$   
 $A_{ij} = \begin{cases} 1 & \text{if } i \sim j \\ 0 & \text{otherwise} \end{cases}$   
 $A \in \mathbb{R}^{n \times n}$   
 $A_{ij} = \begin{cases} 1 & \text{if } i \sim j \\ 0 & \text{otherwise} \end{cases}$

13. Monotone Transformations  
 $f: \mathbb{R}^n \rightarrow \mathbb{R}^n$   
 $f(x) = (f_1(x), \dots, f_n(x))$   
 $f(x) = (f_1(x), \dots, f_n(x))$   
 $f(x) = (f_1(x), \dots, f_n(x))$

14. Asymptotic Expansions  
 $f(x) \sim \sum_{k=0}^{\infty} \frac{a_k}{x^k}$   
 $f(x) \sim \sum_{k=0}^{\infty} \frac{a_k}{x^k}$   
 $f(x) \sim \sum_{k=0}^{\infty} \frac{a_k}{x^k}$

15. Property of vector norm  
 $\|x\| \geq 0$   
 $\|x\| = 0 \iff x = 0$   
 $\|x+y\| \leq \|x\| + \|y\|$   
 $\|\alpha x\| = |\alpha| \|x\|$

16. Matrix norms  
 $\|A\|_1 = \sum_{j=1}^n \sum_{i=1}^m |a_{ij}|$   
 $\|A\|_2 = \sqrt{\lambda_{\max}(A^T A)}$   
 $\|A\|_\infty = \max_{i=1, \dots, m} \sum_{j=1}^n |a_{ij}|$   
 $\|A\|_F = \sqrt{\sum_{i,j} |a_{ij}|^2}$

17. Induced matrix norm  
 $\|A\|_1 = \sum_{j=1}^n \sum_{i=1}^m |a_{ij}|$   
 $\|A\|_2 = \sqrt{\lambda_{\max}(A^T A)}$   
 $\|A\|_\infty = \max_{i=1, \dots, m} \sum_{j=1}^n |a_{ij}|$   
 $\|A\|_F = \sqrt{\sum_{i,j} |a_{ij}|^2}$

18. Induced matrix norm  
 $\|A\|_1 = \sum_{j=1}^n \sum_{i=1}^m |a_{ij}|$   
 $\|A\|_2 = \sqrt{\lambda_{\max}(A^T A)}$   
 $\|A\|_\infty = \max_{i=1, \dots, m} \sum_{j=1}^n |a_{ij}|$   
 $\|A\|_F = \sqrt{\sum_{i,j} |a_{ij}|^2}$

19. Recurrence  
 $x_{n+1} = A x_n + b$   
 $x_n = A^n x_0 + \sum_{k=0}^{n-1} A^k b$   
 $x_n = A^n x_0 + \sum_{k=0}^{n-1} A^k b$

20. Recurrence  
 $x_{n+1} = A x_n + b$   
 $x_n = A^n x_0 + \sum_{k=0}^{n-1} A^k b$   
 $x_n = A^n x_0 + \sum_{k=0}^{n-1} A^k b$

21. Recurrence  
 $x_{n+1} = A x_n + b$   
 $x_n = A^n x_0 + \sum_{k=0}^{n-1} A^k b$   
 $x_n = A^n x_0 + \sum_{k=0}^{n-1} A^k b$

22. Recurrence  
 $x_{n+1} = A x_n + b$   
 $x_n = A^n x_0 + \sum_{k=0}^{n-1} A^k b$   
 $x_n = A^n x_0 + \sum_{k=0}^{n-1} A^k b$

23. Recurrence  
 $x_{n+1} = A x_n + b$   
 $x_n = A^n x_0 + \sum_{k=0}^{n-1} A^k b$   
 $x_n = A^n x_0 + \sum_{k=0}^{n-1} A^k b$

24. Recurrence  
 $x_{n+1} = A x_n + b$   
 $x_n = A^n x_0 + \sum_{k=0}^{n-1} A^k b$   
 $x_n = A^n x_0 + \sum_{k=0}^{n-1} A^k b$

25. Recurrence  
 $x_{n+1} = A x_n + b$   
 $x_n = A^n x_0 + \sum_{k=0}^{n-1} A^k b$   
 $x_n = A^n x_0 + \sum_{k=0}^{n-1} A^k b$

26. Recurrence  
 $x_{n+1} = A x_n + b$   
 $x_n = A^n x_0 + \sum_{k=0}^{n-1} A^k b$   
 $x_n = A^n x_0 + \sum_{k=0}^{n-1} A^k b$

27. Recurrence  
 $x_{n+1} = A x_n + b$   
 $x_n = A^n x_0 + \sum_{k=0}^{n-1} A^k b$   
 $x_n = A^n x_0 + \sum_{k=0}^{n-1} A^k b$

28. Recurrence  
 $x_{n+1} = A x_n + b$   
 $x_n = A^n x_0 + \sum_{k=0}^{n-1} A^k b$   
 $x_n = A^n x_0 + \sum_{k=0}^{n-1} A^k b$

29. Recurrence  
 $x_{n+1} = A x_n + b$   
 $x_n = A^n x_0 + \sum_{k=0}^{n-1} A^k b$   
 $x_n = A^n x_0 + \sum_{k=0}^{n-1} A^k b$

30. Recurrence  
 $x_{n+1} = A x_n + b$   
 $x_n = A^n x_0 + \sum_{k=0}^{n-1} A^k b$   
 $x_n = A^n x_0 + \sum_{k=0}^{n-1} A^k b$

31. Recurrence  
 $x_{n+1} = A x_n + b$   
 $x_n = A^n x_0 + \sum_{k=0}^{n-1} A^k b$   
 $x_n = A^n x_0 + \sum_{k=0}^{n-1} A^k b$

32. Recurrence  
 $x_{n+1} = A x_n + b$   
 $x_n = A^n x_0 + \sum_{k=0}^{n-1} A^k b$   
 $x_n = A^n x_0 + \sum_{k=0}^{n-1} A^k b$

33. Recurrence  
 $x_{n+1} = A x_n + b$   
 $x_n = A^n x_0 + \sum_{k=0}^{n-1} A^k b$   
 $x_n = A^n x_0 + \sum_{k=0}^{n-1} A^k b$

34. Recurrence  
 $x_{n+1} = A x_n + b$   
 $x_n = A^n x_0 + \sum_{k=0}^{n-1} A^k b$   
 $x_n = A^n x_0 + \sum_{k=0}^{n-1} A^k b$

35. Recurrence  
 $x_{n+1} = A x_n + b$   
 $x_n = A^n x_0 + \sum_{k=0}^{n-1} A^k b$   
 $x_n = A^n x_0 + \sum_{k=0}^{n-1} A^k b$

36. Recurrence  
 $x_{n+1} = A x_n + b$   
 $x_n = A^n x_0 + \sum_{k=0}^{n-1} A^k b$   
 $x_n = A^n x_0 + \sum_{k=0}^{n-1} A^k b$

37. Recurrence  
 $x_{n+1} = A x_n + b$   
 $x_n = A^n x_0 + \sum_{k=0}^{n-1} A^k b$   
 $x_n = A^n x_0 + \sum_{k=0}^{n-1} A^k b$

38. Recurrence  
 $x_{n+1} = A x_n + b$   
 $x_n = A^n x_0 + \sum_{k=0}^{n-1} A^k b$   
 $x_n = A^n x_0 + \sum_{k=0}^{n-1} A^k b$

39. Recurrence  
 $x_{n+1} = A x_n + b$   
 $x_n = A^n x_0 + \sum_{k=0}^{n-1} A^k b$   
 $x_n = A^n x_0 + \sum_{k=0}^{n-1} A^k b$

40. Recurrence  
 $x_{n+1} = A x_n + b$   
 $x_n = A^n x_0 + \sum_{k=0}^{n-1} A^k b$   
 $x_n = A^n x_0 + \sum_{k=0}^{n-1} A^k b$

41. Recurrence  
 $x_{n+1} = A x_n + b$   
 $x_n = A^n x_0 + \sum_{k=0}^{n-1} A^k b$   
 $x_n = A^n x_0 + \sum_{k=0}^{n-1} A^k b$

42. Recurrence  
 $x_{n+1} = A x_n + b$   
 $x_n = A^n x_0 + \sum_{k=0}^{n-1} A^k b$   
 $x_n = A^n x_0 + \sum_{k=0}^{n-1} A^k b$

43. Recurrence  
 $x_{n+1} = A x_n + b$   
 $x_n = A^n x_0 + \sum_{k=0}^{n-1} A^k b$   
 $x_n = A^n x_0 + \sum_{k=0}^{n-1} A^k b$

44. Recurrence  
 $x_{n+1} = A x_n + b$   
 $x_n = A^n x_0 + \sum_{k=0}^{n-1} A^k b$   
 $x_n = A^n x_0 + \sum_{k=0}^{n-1} A^k b$

45. Recurrence  
 $x_{n+1} = A x_n + b$   
 $x_n = A^n x_0 + \sum_{k=0}^{n-1} A^k b$   
 $x_n = A^n x_0 + \sum_{k=0}^{n-1} A^k b$

46. Recurrence  
 $x_{n+1} = A x_n + b$   
 $x_n = A^n x_0 + \sum_{k=0}^{n-1} A^k b$   
 $x_n = A^n x_0 + \sum_{k=0}^{n-1} A^k b$

47. Recurrence  
 $x_{n+1} = A x_n + b$   
 $x_n = A^n x_0 + \sum_{k=0}^{n-1} A^k b$   
 $x_n = A^n x_0 + \sum_{k=0}^{n-1} A^k b$

48. Recurrence  
 $x_{n+1} = A x_n + b$   
 $x_n = A^n x_0 + \sum_{k=0}^{n-1} A^k b$   
 $x_n = A^n x_0 + \sum_{k=0}^{n-1} A^k b$



### May 3 PRACTICE PROBLEM

$A_{1010}, B_{1010}, X \in \mathbb{R}^{n \times n}$   
 $(AB)_x = O(n^2) + O(n^2)$   
 $A(Bx) = O(n^2) + O(n^2)$   
 Prob 2:  $\|A\|_1, \|A\|_2, \|A\|_\infty$   
 $\|A\|_1 = \sum_{j=1}^n \sum_{i=1}^n |A_{ij}|$   
 $\|A\|_2 = \sqrt{\lambda_{\max}(A^T A)}$   
 $\|A\|_\infty = \max_{i=1}^n \sum_{j=1}^n |A_{ij}|$   
 Spec:  $\|A\|_1 = \|A^T\|_\infty$   
 Prob 3: Check  $\|A\|_1 = \max_{j=1}^n \sum_{i=1}^n |A_{ij}|$

(1)  $\|A\| \geq 0 \quad \forall A \quad \checkmark$   
 (2)  $\|A\| = 0 \iff A = 0 \quad \checkmark$   
 (3)  $\|cA\| = |c| \|A\| \quad \checkmark$   
 (4)  $\|A+B\| \leq \|A\| + \|B\| \quad \checkmark$   
 (5)  $\|AB\| \leq \|A\| \|B\| \quad \times$   
 $A = \begin{pmatrix} 1 & 1 \\ 1 & 1 \end{pmatrix} \quad B = \begin{pmatrix} 1 & 1 \\ 1 & 1 \end{pmatrix} \quad AB = \begin{pmatrix} 2 & 2 \\ 2 & 2 \end{pmatrix}$   
 But  $\|A\| = \sqrt{2} \quad \|B\| = \sqrt{2} \quad \|AB\| = 2$

$$\begin{aligned} \|A\|_2 &= \sqrt{\lambda_{\max}(A^T A)} \\ &= \sqrt{\sup_{\|x\|_2=1} x^T A^T A x} \\ &= \sqrt{\sup_{\|x\|_2=1} \|Ax\|_2^2} \\ &= \sup_{\|x\|_2=1} \|Ax\|_2 \end{aligned}$$
$$\begin{pmatrix} x'x & x'y \\ x & y \end{pmatrix} \begin{pmatrix} x'x & x'y \\ x & y \end{pmatrix}^{-1} \begin{pmatrix} x'y \\ y \end{pmatrix}$$

$$\begin{pmatrix}
 x'x & x'y \\
 x'p & y'y
 \end{pmatrix}^{-1}
 \begin{pmatrix}
 x'y \\
 x'p & y'y
 \end{pmatrix}$$

$$\begin{pmatrix}
 (x'x)^{-1} & (x'x)^{-1}x'y \\
 (x'p)^{-1} & y'y - x'y(x'x)^{-1}x'y
 \end{pmatrix}$$

$$y - x'y(x'x)^{-1}x'y$$

$$y - y'x'x^{-1}y$$

---

Prob 4:  $\|A\|_F \leq \text{rank}(A)$

$$\|A\|_F^2 = \text{trace}(AA^T)$$

$$\leq \sum \lambda_i$$

$$\leq \sum |\lambda_i|$$

$$\leq m \cdot \max |\lambda_i|$$

$$= \text{rank}(A) \cdot \text{tr}(A)$$

$$\leq \text{rank}(A) \cdot \|A\|_F$$

Prob 5:  $A$  symmetric,  $U$  orthogonal

$$\|U^T A U\|_F^2 = \text{trace}(U^T A U U^T A U)$$

$$= \text{trace}(U^T A^2 U)$$

$$= \text{trace}(A^2)$$

$$= \|A\|_F^2$$

$$\text{trace}(U^T A U) = \text{trace}(A)$$

[illegible][illegible][illegible][illegible]







# HW problems

## HW1 Prob 1:

Define  $g$  subgradient of  $f$  at  $x$  if  $f(y) \geq f(x) + g(y-x)$

Suppose  $g$  is a subgradient of  $f$  at  $x$

Let  $g(x)$  be the 1-th coordinate of  $g(x)$   
 Prove  $g(x) \in [-1, 1]$  and  $g(x) = \text{sgn}(x)$   
 when  $x \neq 0$  for  $i = 1, \dots, n$

$$g_i(x) = \begin{cases} 1 & \text{if } x_i < 0 \\ 0 & \text{if } x_i = 0 \\ -1 & \text{if } x_i > 0 \end{cases}$$

Thus  $g(x) = \text{sgn}(x)$  when  $x \neq 0$

when  $x = 0$ :

$$f(y) \geq f(x) + g(x)(y-x)$$

$$\sum_{i=1}^n y_i - \sum_{i=1}^n x_i \geq g(x)(y-x)$$

$$\sum_{i=1}^n y_i \geq \sum_{i=1}^n g(x)y_i$$

$$1 \geq g(x)$$

$$g(x) \in [-1, 1]$$

$$Q. \text{ Prove } f(x) = \lim_{x \rightarrow 0} \frac{f(x) - f(x_0)}{x - x_0}$$

$$\lim_{x \rightarrow 0} \frac{f(x) - f(x_0)}{x - x_0} = \lim_{x \rightarrow 0} \frac{f(x) - f(x_0)}{x - x_0}$$

$$\Rightarrow f'(x) = \lim_{x \rightarrow 0} \frac{f(x) - f(x_0)}{x - x_0}$$

$$\text{Similarly } x \rightarrow b$$

$$f'(b) = \lim_{x \rightarrow b} \frac{f(x) - f(b)}{x - b}$$

$$d. \text{ Result from } c \text{ implies } f \text{ non-differentiable}$$

$$f'(x_0) = \lim_{h \rightarrow 0} \frac{f(x_0+h) - f(x_0)}{h}$$

$$\text{At } x_0 = a:$$

$$f(a+h) - f(a) \geq 0, h > 0$$

$$\Rightarrow \lim_{h \rightarrow 0^+} \frac{f(a+h) - f(a)}{h} \geq 0$$

$$\Rightarrow f'(a) \geq 0$$

$$\text{Similarly at } x_0 = b$$

$$\lim_{h \rightarrow 0^+} \frac{f(b+h) - f(b)}{h} \geq 0, h < 0$$

$$\Rightarrow f'(b) \geq 0$$

$$Prob 2:$$

$$x^* = \arg \min f(x), f(x) = \sum_{i=1}^n |x_i - x|$$

$$a. \text{ Prove } x^* = \text{median}\{x_1, \dots, x_n\}$$

$$b. \text{ Prove convexity of } f \text{ continuous but not differentiable.}$$

$$c. \text{ Subgradient of } f(x)$$

$$f(x) = \sum_{i=1}^n \text{sgn}(x - x_i)$$

$$b. x_1, x_2 \in \mathbb{R}, \theta \in (0, 1)$$

$$f(\theta x_1 + (1-\theta)x_2) = \sum_{i=1}^n |(\theta x_1 + (1-\theta)x_2) - x_i|$$

$$\leq \theta \sum_{i=1}^n |x_1 - x_i| + (1-\theta) \sum_{i=1}^n |x_2 - x_i|$$

$$= \theta f(x_1) + (1-\theta)f(x_2)$$

$$- f(x) \text{ continuous as its sum of continuous functions}$$

$$- f(x) \text{ not differentiable at } x = x_i$$

$$\text{'kink' at } x_i$$

## Prob 2:

Suppose  $f$  is strictly convex with  $\nabla f(x) = 0$

Let  $A, B$  be a positive definite matrix. Show

$$0 < \lambda \leq \frac{\lambda_{\min}(A+B)}{\lambda_{\min}(A)}$$

Use this to show that  $\nabla f(x) = 0$

$$\text{Recall strongly convex } g(x) = f(x) + \frac{1}{2}x^T Ax$$

$$g(x) - g(0) \leq \frac{1}{2}x^T (A+B)x$$

$$0 \leq x^T (A+B)x \leq \frac{1}{2}x^T (A+B)x$$

$$\Rightarrow 0 < \lambda \leq \frac{\lambda_{\min}(A+B)}{\lambda_{\min}(A)}$$

$$\text{From above, } \nabla f(x) = 0 \Rightarrow \nabla g(x) = 0$$

$$\Rightarrow \nabla f(x) = -\frac{1}{2}Ax$$

$$\Rightarrow \nabla f(x) = 0 \Rightarrow \nabla g(x) = 0$$

$$\Rightarrow \nabla f(x) = 0 \Rightarrow \nabla g(x) = 0$$

$$\Rightarrow \nabla f(x) = 0 \Rightarrow \nabla g(x) = 0$$

$$\Rightarrow \nabla f(x) = 0 \Rightarrow \nabla g(x) = 0$$

$$\Rightarrow \nabla f(x) = 0 \Rightarrow \nabla g(x) = 0$$

$$\Rightarrow \nabla f(x) = 0 \Rightarrow \nabla g(x) = 0$$

$$\Rightarrow \nabla f(x) = 0 \Rightarrow \nabla g(x) = 0$$

$$\Rightarrow \nabla f(x) = 0 \Rightarrow \nabla g(x) = 0$$

$$\Rightarrow \nabla f(x) = 0 \Rightarrow \nabla g(x) = 0$$

$$\Rightarrow \nabla f(x) = 0 \Rightarrow \nabla g(x) = 0$$

$$\Rightarrow \nabla f(x) = 0 \Rightarrow \nabla g(x) = 0$$

$$\Rightarrow \nabla f(x) = 0 \Rightarrow \nabla g(x) = 0$$

$$\Rightarrow \nabla f(x) = 0 \Rightarrow \nabla g(x) = 0$$

$$\Rightarrow \nabla f(x) = 0 \Rightarrow \nabla g(x) = 0$$

$$\Rightarrow \nabla f(x) = 0 \Rightarrow \nabla g(x) = 0$$

$$\Rightarrow \nabla f(x) = 0 \Rightarrow \nabla g(x) = 0$$

$$\Rightarrow \nabla f(x) = 0 \Rightarrow \nabla g(x) = 0$$

$$\Rightarrow \nabla f(x) = 0 \Rightarrow \nabla g(x) = 0$$

$$\Rightarrow \nabla f(x) = 0 \Rightarrow \nabla g(x) = 0$$

$$\Rightarrow \nabla f(x) = 0 \Rightarrow \nabla g(x) = 0$$

$$\Rightarrow \nabla f(x) = 0 \Rightarrow \nabla g(x) = 0$$

$$\Rightarrow \nabla f(x) = 0 \Rightarrow \nabla g(x) = 0$$

$$\Rightarrow \nabla f(x) = 0 \Rightarrow \nabla g(x) = 0$$

$$\Rightarrow \nabla f(x) = 0 \Rightarrow \nabla g(x) = 0$$

$$\Rightarrow \nabla f(x) = 0 \Rightarrow \nabla g(x) = 0$$

$$\Rightarrow \nabla f(x) = 0 \Rightarrow \nabla g(x) = 0$$

$$\Rightarrow \nabla f(x) = 0 \Rightarrow \nabla g(x) = 0$$

$$\Rightarrow \nabla f(x) = 0 \Rightarrow \nabla g(x) = 0$$

$$\Rightarrow \nabla f(x) = 0 \Rightarrow \nabla g(x) = 0$$

$$\Rightarrow \nabla f(x) = 0 \Rightarrow \nabla g(x) = 0$$

$$\Rightarrow \nabla f(x) = 0 \Rightarrow \nabla g(x) = 0$$

## Prob 2:

Show  $f(x) = \log(1+x)$  convex

Using  $f''(x) = \frac{1}{(1+x)^2} > 0$

$$f''(x) = \frac{1}{(1+x)^2} > 0$$

$$f''(x) = \frac{1}{(1+x)^2} > 0$$

$$f''(x) = \frac{1}{(1+x)^2} > 0$$

$$f''(x) = \frac{1}{(1+x)^2} > 0$$

$$f''(x) = \frac{1}{(1+x)^2} > 0$$

$$f''(x) = \frac{1}{(1+x)^2} > 0$$

$$f''(x) = \frac{1}{(1+x)^2} > 0$$

$$f''(x) = \frac{1}{(1+x)^2} > 0$$

$$f''(x) = \frac{1}{(1+x)^2} > 0$$

$$f''(x) = \frac{1}{(1+x)^2} > 0$$

$$f''(x) = \frac{1}{(1+x)^2} > 0$$

$$f''(x) = \frac{1}{(1+x)^2} > 0$$

$$f''(x) = \frac{1}{(1+x)^2} > 0$$

$$f''(x) = \frac{1}{(1+x)^2} > 0$$

$$f''(x) = \frac{1}{(1+x)^2} > 0$$

$$f''(x) = \frac{1}{(1+x)^2} > 0$$

$$f''(x) = \frac{1}{(1+x)^2} > 0$$

$$f''(x) = \frac{1}{(1+x)^2} > 0$$

$$f''(x) = \frac{1}{(1+x)^2} > 0$$

$$f''(x) = \frac{1}{(1+x)^2} > 0$$

$$f''(x) = \frac{1}{(1+x)^2} > 0$$

$$f''(x) = \frac{1}{(1+x)^2} > 0$$

$$f''(x) = \frac{1}{(1+x)^2} > 0$$

$$f''(x) = \frac{1}{(1+x)^2} > 0$$

$$f''(x) = \frac{1}{(1+x)^2} > 0$$

$$f''(x) = \frac{1}{(1+x)^2} > 0$$

$$f''(x) = \frac{1}{(1+x)^2} > 0$$

$$f''(x) = \frac{1}{(1+x)^2} > 0$$

$$f''(x) = \frac{1}{(1+x)^2} > 0$$

$$f''(x) = \frac{1}{(1+x)^2} > 0$$

$$f''(x) = \frac{1}{(1+x)^2} > 0$$

$$f''(x) = \frac{1}{(1+x)^2} > 0$$

$$f''(x) = \frac{1}{(1+x)^2} > 0$$

$$f''(x) = \frac{1}{(1+x)^2} > 0$$

$$f''(x) = \frac{1}{(1+x)^2} > 0$$

$$f''(x) = \frac{1}{(1+x)^2} > 0$$

$$f''(x) = \frac{1}{(1+x)^2} > 0$$

$$f''(x) = \frac{1}{(1+x)^2} > 0$$

$$f''(x) = \frac{1}{(1+x)^2} > 0$$

## HW1 Prob 1:

Let  $A, B$  and  $C$  be the normalized

and unnormalized vectors

$$\|A\|_2 = \sqrt{\lambda_{\max}(A^T A)}$$

$$\|B\|_2 = \sqrt{\lambda_{\max}(B^T B)}$$

$$\|C\|_2 = \sqrt{\lambda_{\max}(C^T C)}$$

$$\|A\|_2 = \sqrt{\lambda_{\max}(A^T A)}$$

$$\|B\|_2 = \sqrt{\lambda_{\max}(B^T B)}$$

$$\|C\|_2 = \sqrt{\lambda_{\max}(C^T C)}$$

$$\|A\|_2 = \sqrt{\lambda_{\max}(A^T A)}$$

$$\|B\|_2 = \sqrt{\lambda_{\max}(B^T B)}$$

$$\|C\|_2 = \sqrt{\lambda_{\max}(C^T C)}$$

$$\|A\|_2 = \sqrt{\lambda_{\max}(A^T A)}$$

$$\|B\|_2 = \sqrt{\lambda_{\max}(B^T B)}$$

$$\|C\|_2 = \sqrt{\lambda_{\max}(C^T C)}$$

$$\|A\|_2 = \sqrt{\lambda_{\max}(A^T A)}$$

$$\|B\|_2 = \sqrt{\lambda_{\max}(B^T B)}$$

$$\|C\|_2 = \sqrt{\lambda_{\max}(C^T C)}$$

$$\|A\|_2 = \sqrt{\lambda_{\max}(A^T A)}$$

$$\|B\|_2 = \sqrt{\lambda_{\max}(B^T B)}$$

$$\|C\|_2 = \sqrt{\lambda_{\max}(C^T C)}$$

$$\|A\|_2 = \sqrt{\lambda_{\max}(A^T A)}$$

$$\|B\|_2 = \sqrt{\lambda_{\max}(B^T B)}$$

$$\|C\|_2 = \sqrt{\lambda_{\max}(C^T C)}$$

$$\|A\|_2 = \sqrt{\lambda_{\max}(A^T A)}$$

$$\|B\|_2 = \sqrt{\lambda_{\max}(B^T B)}$$

$$\|C\|_2 = \sqrt{\lambda_{\max}(C^T C)}$$

$$\|A\|_2 = \sqrt{\lambda_{\max}(A^T A)}$$

$$\|B\|_2 = \sqrt{\lambda_{\max}(B^T B)}$$

$$\|C\|_2 = \sqrt{\lambda_{\max}(C^T C)}$$

$$\|A\|_2 = \sqrt{\lambda_{\max}(A^T A)}$$

$$\|B\|_2 = \sqrt{\lambda_{\max}(B^T B)}$$

$$\|C\|_2 = \sqrt{\lambda_{\max}(C^T C)}$$

$$\|A\|_2 = \sqrt{\lambda_{\max}(A^T A)}$$

$$\|B\|_2 = \sqrt{\lambda_{\max}(B^T B)}$$

$$\|C\|_2 = \sqrt{\lambda_{\max}(C^T C)}$$

$$\|A\|_2 = \sqrt{\lambda_{\max}(A^T A)}$$

$$\|B\|_2 = \sqrt{\lambda_{\max}(B^T B)}$$

$$\|C\|_2 = \sqrt{\lambda_{\max}(C^T C)}$$

$$\|A\|_2 = \sqrt{\lambda_{\max}(A^T A)}$$

$$\|B\|_2 = \sqrt{\lambda_{\max}(B^T B)}$$

$$\|C\|_2 = \sqrt{\lambda_{\max}(C^T C)}$$